trace: incorporate policy transition into trace

theories/security.v
@@ -1,12 +1,13 @@
 Require Import List.
+Require Import Logic.Eqdep_dec Logic.EqdepFacts.
 Require Import Unicode.Utf8.
 
 Require Import config.
 Require Import data_model.
 Require Import lattice.
-Require Import prov.
 Require Import relation.
 Require Import semantics.
+Require Import trace.
 Require Import types.
 Require Import util.
 
@@ -19,106 +20,144 @@ Definition can_release p: Prop := p = ∎.
 (* TODO: Define this. *)
 Definition budget_bounded (β: budget): Prop := True.
 
-Definition valid_transition (τ: prov_type) (p1 p2: Policy.policy): Prop :=
-  p1 ⪯ p2 ∧
-  match τ with
-    | prov_trans_unary op => (∘ (Policy.policy_transform ((unary_trans_op op) :: nil))) ⪯ p1
-    | prov_trans_binary op => (∘ (Policy.policy_transform ((binary_trans_op op) :: nil))) ⪯ p1
-    | prov_agg op => (∘ (Policy.policy_agg (op :: nil))) ⪯ p1
-    | prov_noise op => (∘ (Policy.policy_noise op)) ⪯ p1
-    | prov_join => True
-  end.
+(*
+ * Rules for the valid label transition.
+ *)
+Inductive downgrade_ok: prov_type → Policy.policy → Policy.policy → Prop :=
+  | DowngradeUnary: ∀ prov op p1 p2,
+      p2 ⪯ p1 →
+      prov = prov_trans_unary op →
+      downgrade_ok prov p1 p2
+.
+
+(* TODO: Implement this. *)
+Notation "p1 '=[' p ']=>' p2" := (downgrade_ok p p1 p2)
+  (at level 10, p at next level, p2 at next level).
+
+Inductive join_ok: Policy.policy → trace_ty → trace_ty → Prop :=
+  | JoinOk: ∀ lbl lbl1 lbl2 tr1 tr2,
+      lbl1 = extract_policy tr1 →
+      lbl2 = extract_policy tr2 →
+      lbl1 ⪯ lbl →
+      lbl2 ⪯ lbl →
+      join_ok lbl tr1 tr2
+.
 
 (*
-  @param c1 The initial policy context.
-  @param c2 The final policy context.
-  @param p The policy that is being checked.
-  @param prov_ctx The provenance context.
-  @param prov The provenance tree that is being checked.
-  @return A proposition that is true if the provenance tree is valid and false otherwise.
-
-  Checks whether a given provenance tree (consisting of cells) is valid in the course of a query execution.
-  It checks if policies are correctly enforced and if all transitions are permitted.
-*)
-Inductive prov_ok: Policy.context → Policy.context → Policy.policy → prov_ctx → prov → Prop :=
-  | prov_ok_none: ∀ Γ Γ' ε' p, prov_ok Γ Γ' ε' p prov_none
-  | prov_ok_list: ∀ Γ Γ' ε' p prv τ l,
-      prv = prov_list τ l →
-      prov_list_ok Γ Γ' ε' p τ l →
-      prov_ok Γ Γ' ε' p prv
-  with
-prov_list_ok: Policy.context → Policy.context → Policy.policy → prov_ctx → prov_type → list (nat * prov) → Prop :=
-  | prov_list_ok_empty: ∀ Γ Γ' ε' p τ, prov_list_ok Γ Γ' ε' p τ nil
-  | prov_list_ok_cons: ∀ Γ Γ' ε ε' p τ c prov l l',
-      l = (c, prov) :: l' →
-      label_lookup Γ c  = Some ε →
-      can_release ε →
-      valid_transition τ ε ε' →
-      prov_list_ok Γ Γ' ε' p τ l' →
-      prov_ok Γ Γ' ε' p prov →
-      prov_list_ok Γ Γ' ε' p τ l
+ * The dependency graph:
+ *
+ * label_transition_valid --> label_transition_valid_impl --> valid_transition
+ *  ^                                                               |
+ *  |                                                               |
+ *  +---------------------------------------------------------------+
+ *)
+Inductive label_transition_valid: trace_ty → Prop :=
+  | LabelTransitionTrEmpty: label_transition_valid ∅
+  | LabelTransitionTrLinear: ∀ tr prov lbl l,
+      tr = TrLinear prov lbl l →
+      label_transition_valid_impl prov lbl l →
+      label_transition_valid tr
+  | LabelTransitionTrBranch: ∀ tr lbl prov tr1 tr2,
+      tr = TrBranch prov lbl tr1 tr2 →
+      label_transition_valid tr1 →
+      label_transition_valid tr2 →
+      join_ok lbl tr1 tr2 →
+      label_transition_valid tr
+(*
+ * Checks against the list element, can it be released via the current label?
+ *)
+with
+label_transition_valid_impl: prov_type → Policy.policy → list (trace_ty) → Prop :=
+  | LabelTransitionImplNil: ∀ prov lbl, label_transition_valid_impl prov lbl nil
+  | LabelTransitionImplCons: ∀ prov lbl tr hd tl,
+      tr = hd :: tl →
+      label_transition_valid_impl prov lbl tl →
+      valid_transition prov lbl hd →
+      label_transition_valid_impl prov lbl (hd :: tl)
+(*
+ * Checks against for each element, can it be released via the current label?
+ *)
+with
+valid_transition: prov_type → Policy.policy → trace_ty → Prop :=
+  | ValidEmpty: ∀ prov lbl, valid_transition prov lbl ∅
+  | ValidTransition: ∀ prov lbl lbl' tr,
+      lbl' = extract_policy tr →
+      lbl =[ prov ]=> lbl' →
+      valid_transition prov lbl tr
 .
 
-Inductive label_transition_valid_es: Policy.context → Policy.context → prov_ctx → list nat → Prop :=
-  | label_valid_empty_list: ∀ Γ Γ' p, label_transition_valid_es Γ Γ' p nil
-  | label_valid_transition: ∀ Γ Γ' p c lc lc' ε ε' prov_term,
-      lc = c :: lc' →
-      label_lookup Γ c = Some ε →
-      label_lookup Γ' c = Some ε' →
-      can_release ε →
-      label_lookup p c = Some (prov_term) →
-      prov_ok Γ Γ' ε' p prov_term →
-      label_transition_valid_es Γ Γ' p lc' →
-      label_transition_valid_es Γ Γ' p lc
+(*
+ * We iterate over the trace information and checks for each cell id if its
+ * corresponding policy transition is indeed valid and enforced in the course of
+ * the query execution trace.
+ *)
+Inductive trace_ok: trace → Prop :=
+  | TraceEmpty: trace_ok nil
+  | TraceCons: ∀ tr hd tl,
+      tr = hd :: tl →
+      label_transition_valid (snd hd) →
+      trace_ok tl →
+      trace_ok (hd :: tl)
 .
 
-Inductive label_transition_valid: ∀ s, relation s → Policy.context → Policy.context → prov_ctx → Prop :=
-  | valid_refl: ∀ s r Γ p, label_transition_valid s r Γ Γ p
-  | valid_empty_schema: ∀ s r Γ Γ' p, s = nil → label_transition_valid s r Γ Γ' p
-  | valid_env: ∀ s r r' Γ Γ' p, s ≠ nil →
-      r' = extract_as_cell_list s r →
-      label_transition_valid_es Γ Γ' p r' →
-      label_transition_valid s r Γ Γ' p
-.
-
-(* 
+(*
     ∀Γ, Γ′.Γ −→ Γ′ =⇒ ∀c′ ∈ Γ′.ℓ′1 ⊑ ℓ =⇒
       ∃C = {c1, · · · cn} −→ c′ =⇒
         ∀c ∈ C.(ℓ1, ℓ2) = Γ(c) ∧ ℓ1 ⊑ ℓ2 =⇒ Ok(ℓ1 ⇝o ℓ′1)
 
     Should we start from empty environment? Or this condition is unnecessary?
  *)
+
+(*
+ * This theorem is the main security theorem that states the following fact:
+ *
+ * Given an initial environment where the configuration is valid, one of the followings holds:
+ * * The query evaluation results in an error, or
+ * * There exists some configuration such that the query evaluation results in that configuration
+ *   and the label transition is valid with regard to the cell provenance information, and that
+ *   the budget is bounded.
+ *
+ * The proof is by induction on `o`.
+ *
+ * Note here we do not enforce how the data should be released, we only ensure that all the valid
+ * transitions are enforced and that the budget is bounded. The release of data can be trivally
+ * enforced by an extra epilogue function. The proof for that function is not included here.
+ *)
 Theorem secure_query:
-  ∀ c db Γ β p o,
-  c = ⟨ db Γ β p ⟩ ∧ config_valid c →
-  ⟦ c o ⟧ ⇓ ⟦ config_error ⟧ ∨
-    (∃ s c' db' Γ' β' p' r, 
-        c' = config_output (RelationWrapped s r) (⟨ db' Γ' β' p' ⟩) →
-      ⟦ c o ⟧ ⇓ ⟦ c' ⟧ ∧ label_transition_valid s r Γ Γ' p' ∧ budget_bounded β').
+  ∀ db o, ⟦ db o ⟧ ⇓ ⟦ ConfigError ⟧ ∨
+    (∃ s c r σ tr,
+      (* The output is valid. *)
+      c = ConfigOut (RelationWrapped s r) σ tr ∧
+      (* The evalaution goes to c. *)
+      ⟦ db o ⟧ ⇓ ⟦ c ⟧ ∧
+      (* The transition of the trace is also valid. *)
+      trace_ok tr ∧ budget_bounded (snd σ)).
 Proof.
-  induction o; intros; destruct H.
+  (* induction o; intros; destruct H.
   - right.
-    exists nil, (config_output (RelationWrapped nil nil) c), db, Γ, β, p, nil. split.
+    exists nil, (ConfigOut (RelationWrapped nil nil) c), db, Γ, β, p, nil. split.
     + specialize E_Empty with
-      (c := c) (c' := config_output (RelationWrapped nil nil) c) (db := db) (Γ := Γ) (β := β) (p := p).
-      intros. intuition. subst. apply H2.
-    + constructor.
-      * constructor.
-      * red. trivial.
+      (c := c) (c' := ConfigOut (RelationWrapped nil nil) c) (db := db) (Γ := Γ) (β := β) (p := p).
+      intros. intuition. subst. auto.
+    + split.
+      * subst. apply E_Empty with (c := ⟨ db Γ β p ⟩); auto.
+      * split; constructor.
   - destruct db eqn: Hdb.
     + left. eapply E_GetRelationDbEmpty; subst; eauto.
     + destruct (database_get_contexts db n) as [ [ [ r' Γ' ] p' ] | ] eqn: Hget.
-      * destruct r'. right. exists s0, (⟨ db Γ' β p' ⟩), db, Γ', β, p', r. split.
+      * destruct r'. right.
+        exists s0, (ConfigOut (RelationWrapped s0 r) (⟨ db Γ' β p' ⟩)), db, Γ', β, p', r.
+        split; split; auto.
         -- eapply E_GetRelation with (db := db) (o := OperatorRel n).
           ++ red. intros. rewrite Hdb in H1. inversion H1.
           ++ reflexivity.
           ++ rewrite <- Hdb in H. eapply H.
           ++ eapply Hget.
-          ++ eapply H1.
+          ++ auto.
         -- split; simpl.
           ++ destruct s0.
             ** constructor. reflexivity.
-            ** inversion H1.
+            ** 
           ++ inversion H1.
       * left. eapply E_GetRelationError with (db := db) (Γ := Γ) (β := β) (p := p); eauto.
         -- red. intros. subst. inversion H1.
@@ -136,11 +175,11 @@ Proof.
       * eapply H4.
       * eapply H5.
       * intuition.
-    + assert (c ≠ config_error) by (subst; try discriminate). intuition. destruct H1.
+    + assert (c ≠ ConfigError) by (subst; try discriminate). intuition. destruct H1.
       left. eapply E_UnionError; eauto.
-    + assert (c ≠ config_error) by (subst; try discriminate). intuition. destruct H6.
+    + assert (c ≠ ConfigError) by (subst; try discriminate). intuition. destruct H6.
       left. eapply E_UnionError; eauto.
-    + assert (c ≠ config_error) by (subst; try discriminate). intuition.
+    + assert (c ≠ ConfigError) by (subst; try discriminate). intuition.
       destruct H1; destruct H6; destruct x0; destruct x; subst; try discriminate; intuition.
       * left. eapply E_UnionError; eauto.
       * left. eapply E_UnionError; eauto.
@@ -153,7 +192,7 @@ Proof.
       * destruct r; destruct r0; destruct x0; destruct x.
         -- inversion H1; subst; try discriminate.
         -- inversion H2; subst; try discriminate.
-        -- inversion H1; subst; try discriminate.
+        -- inversion H2; subst; try discriminate.
         -- inversion H1; subst; try discriminate.
         -- right.
           (* Now we need to discuss the equality of two schemas. *)
@@ -162,7 +201,7 @@ Proof.
             pose (merged_p := merge_env p0 p1).
             pose (merged_Γ := merge_env c c0).
             pose (merged_β := calculate_budget b b0).
-            exists s0, (config_output (RelationWrapped _ (r ++ r0)) (⟨ d0 merged_Γ merged_β merged_p ⟩)),
+            exists s0, (ConfigOut (RelationWrapped _ (r ++ r0)) (⟨ d0 merged_Γ merged_β merged_p ⟩)),
                    d0, merged_Γ, merged_β, merged_p, (r ++ r0).
             intros. split.
             ** econstructor; eauto.
@@ -174,7 +213,9 @@ Proof.
                   *** intuition. discriminate.
                   *** eauto.
                   *** constructor.
-                +++ (* Introduce te existential variable from hypothesis. *)
-            
-
+                +++ 
+                  (* Introduce the existential variable from hypothesis. *)
+                  destruct H5 as [s'1 [c'1 [db'1 [Γ'1 [β'1 [p'1 [r'1 H5'] ] ] ] ] ] ].
+                  destruct H4 as [s'2 [c'2 [db'2 [Γ'2 [β'2 [p'2 [r'2 H4'] ] ] ] ] ] ]. *)
+                  
 Admitted.
