theories/trace.v
@@ -1,0 +1,57 @@
+Require Import List.
+Require Import Unicode.Utf8.
+
+Require Import data_model.
+Require Import types.
+Require Import util.
+
+Inductive prov_type: Set :=
+  | prov_trans_unary: un_op → prov_type
+  | prov_trans_binary: bin_op → prov_type
+  | prov_agg: agg_op → prov_type
+  | prov_noise: noise_op → prov_type
+  | prov_join: prov_type
+.
+
+Definition prov_type_eqb τ1 τ2: bool :=
+  match τ1, τ2 with
+  | prov_trans_unary op1, prov_trans_unary op2 => un_op_eqb op1 op2
+  | prov_trans_binary op1, prov_trans_binary op2 => bin_op_eqb op1 op2
+  | prov_agg op1, prov_agg op2 => agg_op_eqb op1 op2
+  | prov_noise op1, prov_noise op2 => noise_op_eqb op1 op2
+  | prov_join, prov_join => true
+  | _, _ => false
+  end.
+
+Inductive trace_ty: Type :=
+  (* ⊥ *)
+  | TrEmpty: trace_ty
+  (* Linear trace: op → current policy → predecessors *)
+  | TrLinear: prov_type → Policy.policy → list trace_ty → trace_ty
+  (* Branching trace. *)
+  | TrBranch: prov_type → Policy.policy → trace_ty → trace_ty → trace_ty
+.
+
+Definition extract_policy tr :=
+  match tr with
+  | TrEmpty => ∎
+  | TrLinear _ p _ => p
+  | TrBranch _ p _ _ => p
+  end.
+
+(*
+ * A trace is a list of tuples recording how a given data cell is transitioned
+ * from one policy to another; it also bookkeeps the provenance information.
+ *)
+Definition trace := ctx trace_ty.
+
+Fixpoint empty_trace_from_pctx (Γ: Policy.context): trace :=
+  match Γ with
+  | nil => nil
+  | (n, _) :: Γ' => (n, TrEmpty) :: empty_trace_from_pctx Γ'
+  end.
+
+(* σ ::= ⟨ Γ, β ⟩; the program state. *)
+Definition σ := (Policy.context * budget)%type.
+
+Notation "∅" := TrEmpty.
